theories/partial/choice.v
@@ -1,0 +1,261 @@
+Require Import Classical.
+Require Import FunctionalExtensionality.
+
+Section existT_inj2_uip.
+  Variables (A : Type) (P : A -> Type).
+
+  Implicit Type (x : A).
+  Print sigT.
+
+  Theorem exist_inj2_helper x (px : P x) (y : sigT P) :
+      @existT _ _ x px = y
+    -> exists e : x = projT1 y, eq_rect x P px _ e = projT2 y.
+  Proof using Type. intros []; exists eq_refl; auto. Qed.
+
+  Fact exists_inj2 x y (px : P x) (py : P y) :
+      existT _ x px = existT _ y py
+    -> exists e : x = y, eq_rect x P px _ e = py.
+  Proof using Type. intros (e & ?)%exist_inj2_helper. exists e; subst; simpl; auto. Qed.
+
+  Fact exist_inj2_uip :
+    forall x (p1 p2 : P x), existT _ x p1 = existT _ x p2 -> p1 = p2.
+  Proof using Type.
+    intros x p1 p2 (e & He)%exists_inj2.
+    rewrite (UIP _ _ _ e eq_refl) in He.
+    assumption.
+  Qed.
+End existT_inj2_uip.
+
+(* These are how it works in the lean4 standard library *)
+Axiom choose : forall (T : Type) (P : T -> Prop), (exists t, P t) -> T.
+Axiom chooseSpec : forall T P x, P (choose T P x).
+(* Apparently by Diaconescu's theorem you can derive LEM from this (see lean stdlib) *)
+
+Theorem choiceInd : forall (T : Type) (P Q : T -> Prop) x,
+    (forall t, P t -> Q t) -> Q (choose T P x).
+Proof.
+  intros.
+  apply H.
+  apply chooseSpec.
+Qed.
+
+Definition Pif {A : Type} (P : Prop) (a1 a2 : A) : A.
+  Search (Prop -> Type).
+  Check (sum {a : A | P} {a : A | ~ P}).
+  refine (choose A (fun a => P /\ a = a1 \/ ~P /\ a = a2) _).
+  destruct (classic P).
+  - exists a1.
+    auto.
+  - exists a2.
+    auto.
+Defined.
+
+Theorem PifDef1 : forall (A : Type) P (a1 a2 : A), P -> Pif P a1 a2 = a1.
+Proof.
+  intros.
+  unfold Pif.
+  evar (exists t : A, P /\ t = a1 \/ ~ P /\ t = a2).
+  destruct (chooseSpec A (fun a : A => P /\ a = a1 \/ ~ P /\ a = a2) e).
+  - destruct H0.
+    unfold e in H1.
+    erewrite H1.
+    reflexivity.
+  - destruct H0.
+    contradiction.
+Qed.
+
+Theorem PifDef2 : forall (A : Type) P (a1 a2 : A), ~P -> Pif P a1 a2 = a2.
+Proof.
+  intros.
+  unfold Pif.
+  apply choiceInd.
+  intros.
+  destruct H0.
+  - destruct H0.
+    contradiction.
+  - destruct H0.
+    assumption.
+Qed.
+
+Check choose.
+(* Using choice, returns the element of T satisfying P if it exists, otherwise None *)
+Definition chooseOption (T : Type) (P : T -> Prop) : option T.
+  refine (choose (option T)
+                 (fun ot => ((~exists t, P t) /\ ot = None) \/ (exists t, P t /\ ot = Some t)) _).
+  destruct (classic (exists t, P t)).
+  - destruct H.
+    exists (Some x).
+    apply or_intror.
+    eauto.
+  - exists None.
+    apply or_introl.
+    eauto.
+Defined.
+
+Theorem chooseOptionSpec1 : forall T P t,
+    chooseOption T P = Some t -> P t.
+Proof.
+  intros T P t.
+  unfold chooseOption.
+  apply choiceInd.
+  intros.
+  destruct H.
+  - destruct H.
+    subst.
+    inversion H0.
+  - destruct H.
+    destruct H.
+    subst.
+    inversion H0.
+    subst.
+    assumption.
+Qed.  
+
+Theorem chooseOptionSpec2 : forall T P,
+    chooseOption T P = None -> ~exists t, P t.
+Proof.
+  intros T P.
+  unfold chooseOption.
+  apply choiceInd.
+  intros.
+  destruct H.
+  - destruct H.
+    assumption.
+  - destruct H.
+    destruct H.
+    subst.
+    inversion H0.
+Qed.
+    
+Definition collectOption {A B : Type} (f : A -> option B) : option (A -> B) :=
+  (chooseOption (A -> B) (fun f' => forall a, (Some (f' a)) = f a)).
+
+Definition collectOption2 {A : Type} {B : A -> Type} {C : Type}
+           (f : forall (a : A), B a -> option C) : option (forall a, B a -> C) :=
+  chooseOption (forall a, B a -> C) (fun f' => forall a b, Some (f' a b) = f a b).
+
+(* Is this really not in the standard library? *)
+Definition bind {A B : Type} (a : option A) (f : A -> option B) : option B :=
+  match a with
+  | Some a' => f a'
+  | None => None
+  end.
+
+Inductive Prog (A B : Type) : Type :=
+| Ret : option B -> Prog A B
+| Rec : forall (P : A -> Prop), ((forall a, P a -> B) -> Prog A B) -> Prog A B
+.
+
+Inductive runProgR {A B : Type} (def : A -> Prog A B) : Prog A B -> B -> Prop :=
+| retR : forall b, runProgR def (Ret _ _ (Some b)) b
+| recR : forall P (recVals : forall a, P a -> B)
+                 (res : B) (rest : (forall a, P a -> B) -> Prog A B),
+    (* if for all inputs a satisfying P, recVals describes the recursive calls *)
+    (forall a (pa : P a), runProgR def (def a) (recVals a pa))
+    (* and given the results of those recursive calls, the program outputs res *)
+    -> runProgR def (rest recVals) res
+    (* then overall res *)
+    -> runProgR def (Rec _ _ P rest) res
+.
+
+Theorem runProgFunction {A B : Type} {def : A -> Prog A B} {p : Prog A B} {b1 b2 : B}
+  (rp1 : runProgR def p b1) (rp2 : runProgR def p b2) : b1 = b2.
+Proof.
+  intros.
+  generalize rp2.
+  generalize b2.
+  clear rp2.
+  clear b2.
+  induction rp1.
+  - intros.
+    inversion rp2.
+    reflexivity.
+  - intros.
+    inversion rp2.
+    subst.
+    apply IHrp1.
+    assert (rest1 = rest). {
+      apply exist_inj2_uip in H2.
+      assumption.
+    }
+    subst.
+    assert (recVals = recVals0). {
+      extensionality a.
+      extensionality pa.
+      specialize (H a pa).
+      specialize (H3 a pa).
+      apply H0.
+      apply H3.
+    }
+    subst.
+    assumption.
+Qed.
+
+Definition runProgImpl {A B : Type} (def : A -> Prog A B) (p : Prog A B) : option B.
+  Check Pif.
+  Check choose.
+  refine (choose (option B) (fun ob =>
+                               (exists b, runProgR def p b /\ ob = Some b)
+                               \/
+                                 (ob = None /\ ~exists b, runProgR def p b)) _).
+  destruct (classic (exists b, runProgR def p b)).
+  - destruct H.
+    exists (Some x).
+    apply or_introl.
+    eauto.
+  - exists None.
+    apply or_intror.
+    eauto.
+Defined.
+
+Definition runProg {A B : Type} (def : A -> Prog A B) (a : A) : option B :=
+  (runProgImpl def (def a)).
+
+Theorem runProgDefinitionRet {A B : Type} (def : A -> Prog A B) (b : B)
+  : runProgImpl def (Ret _ _ (Some b)) = Some b.
+  intros.
+  unfold runProgImpl.
+  apply choiceInd.
+  intros.
+  destruct H.
+  - destruct H as [b0 [H1 H2]].
+    inversion H1.
+    subst.
+    reflexivity.
+  - destruct H.
+    exfalso.
+    apply H0.
+    exists b.
+    constructor.
+Qed.
+Check collectOption.
+
+Theorem runProgDefinitionRec {A B : Type} {def : A -> Prog A B}
+        {P : A -> Prop}
+        {rest : (forall a, P a -> B) -> Prog A B}
+  : runProgImpl def (Rec _ _ P rest) =
+      bind ((collectOption2 (fun a pa => runProg def a)) : option (forall a, P a -> B))
+           (fun f => runProgImpl def (rest f)).
+Proof.
+  repeat unfold runProgImpl, runProg, collectOption2, chooseOption.
+  repeat apply choiceInd.
+  intros.
+
+(*
+Theorem runProgDefinitionRec2 {A B : Type} {def : A -> Prog A B}
+        {P : A -> Prop}
+        {rest : (forall a, P a -> B) -> Prog A B}
+        {recVals : forall a, P a -> B}
+        (recValsCorrect : forall a (pa : P a), runProg3 def a = Some (recVals a pa))
+  : runProgImpl def (Rec3 _ _ P rest) = runProgImpl def (rest recVals).
+Proof.
+  unfold runProgImpl at 1.
+  apply choiceInd.
+  intros.
+  destruct H.
+  - destruct H.
+    destruct H.
+    subst.
+    unfold runProg3 in recValsCorrect.
+    rewrite
+*)
