theories/partial/coinductive.v
@@ -1,0 +1,284 @@
+Require Import FunctionalExtensionality.
+Require Import Coq.Logic.PropExtensionality.
+Require Import Coq.Logic.ProofIrrelevance.
+
+(*
+Is it possible that a coinductive type could allow me to define recursive functions which make an infinite number of recursive calls?
+
+LATER: Yes, but you can't do match on QTerm with coinductive, which you can with Partial.
+*)
+
+(* basic version without multibind from https://www21.in.tum.de/~krauss/papers/recursion.pdf *)
+CoInductive Computation : forall (A : Type), Type :=
+| ret : forall A, A -> Computation A
+| bind : forall A B, Computation A -> (A -> Computation B) -> Computation B
+| multibind : forall A B I,
+    (I -> Computation A)
+    -> ((I -> A) -> Computation B)
+    -> Computation B
+.
+
+CoFixpoint fancyid (n : nat) : Computation nat :=
+  match n with
+  | O => ret _ 0
+  | S m => bind _ _ (fancyid m) (fun res => ret _ (1 + res))
+  end.
+
+
+(*
+f : nat * nat -> Prop
+f (0, _) = True
+f (n, S m) = not (forall n', f (n', m))
+ *)
+
+CoFixpoint f (n : nat) (m : nat) : Computation Prop :=
+  match m with
+  | O => ret _ True
+  | S m' => multibind _ _ nat (fun n' => f n' m') (fun rec => ret _ (not (forall n', rec n')))
+  end.
+
+(* It seems to work ?! *)
+
+
+Inductive eval : forall {A}, Computation A -> A -> Prop :=
+| eval_ret : forall A a, eval (ret A a) a
+| eval_bind : forall A B ca a f res,
+    eval ca a
+    -> eval (f a) res
+    -> eval (bind A B ca f) res
+| eval_multibind : forall A B I cas aa f res,
+    (forall i, eval (cas i) (aa i))
+    -> eval (f aa) res
+    -> eval (multibind A B I cas f) res
+.
+
+
+(*This section is from https://proofassistants.stackexchange.com/questions/4696/how-to-extract-the-equality-between-the-second-projection-in-an-existential-in-c*)
+(* TODO: Is there really no easier way? Does this really require UIP? *)
+Section existT_inj2_uip.
+  Variables (A : Type) (P : A -> Type).
+
+  Implicit Type (x : A).
+  Print sigT.
+
+  Theorem exist_inj2_helper x (px : P x) (y : sigT P) :
+      @existT _ _ x px = y
+    -> exists e : x = projT1 y, eq_rect x P px _ e = projT2 y.
+  Proof using Type. intros []; exists eq_refl; auto. Qed.
+
+  Fact exists_inj2 x y (px : P x) (py : P y) :
+      existT _ x px = existT _ y py
+    -> exists e : x = y, eq_rect x P px _ e = py.
+  Proof using Type. intros (e & ?)%exist_inj2_helper. exists e; subst; simpl; auto. Qed.
+
+  Fact exist_inj2_uip :
+    forall x (p1 p2 : P x), existT _ x p1 = existT _ x p2 -> p1 = p2.
+  Proof using Type.
+    intros x p1 p2 (e & He)%exists_inj2.
+    rewrite (UIP _ _ _ e eq_refl) in He.
+    assumption.
+  Qed.
+End existT_inj2_uip.
+
+Theorem eval_function {A} (c : Computation A) (a1 a2 : A)
+  : eval c a1 -> eval c a2 -> a1 = a2.
+Proof.
+  intros.
+  generalize dependent H0.
+  induction H.
+  - intros.
+    inversion H0.
+    apply exist_inj2_uip in H2, H3.
+    subst.
+    reflexivity.
+  - intros.
+    inversion H1.
+    subst.
+    apply exist_inj2_uip in H3, H6, H7, H6.
+    subst.
+    apply IHeval2.
+    rewrite (IHeval1 _ H5).
+    assumption.
+  - intros.
+    inversion H2.
+    subst.
+    apply exist_inj2_uip in H8, H7, H9, H8, H8, H7.
+    subst.
+    apply IHeval.
+    assert (aa = aa0). {
+      extensionality i.
+      apply H0.
+      apply H6.
+    }
+    subst.
+    assumption.
+Qed.
+
+Theorem bindDef : forall A B a f,
+    eval (bind A B (ret A a) f) = eval (f a).
+Proof.
+  intros.
+  extensionality b.
+  apply propositional_extensionality.
+  split.
+  - intros.
+    inversion H.
+    clear H.
+    subst.
+    apply exist_inj2_uip in H1, H4, H5, H4.
+    subst.
+    Check (eval_bind).
+    inversion H3.
+    apply exist_inj2_uip in H1, H2.
+    subst.
+    assumption.
+  - intros.
+    eapply eval_bind.
+    + constructor.
+    + apply H.
+Qed.
+
+Theorem multibindDef : forall A B I (rec : I -> A) f,
+    eval (multibind A B I (fun i => ret A (rec i)) f) = eval (f rec).
+Proof.
+  intros.
+  extensionality b.
+  apply propositional_extensionality.
+  split.
+  - intros.
+    inversion H.
+    clear H.
+    subst.
+    apply exist_inj2_uip in H5, H4, H5, H4, H5, H6.
+    subst.
+    Check (eval_bind).
+    assert (rec = aa). {
+      extensionality i.
+      specialize (H3 i).
+      inversion H3.
+      apply exist_inj2_uip in H1, H2.
+      subst.
+      assumption.
+    }
+    subst.
+    assumption.
+  - intros.
+    eapply eval_multibind.
+    + constructor.
+    + apply H.
+Qed.    
+
+(*
+Need it to be an equivalence, and also injectivity (ceq (ret x) (ret y)) -> x = y.
+*)
+
+(* This definition needs funext and propext to make sense *)
+Definition ceq {A} (c1 c2 : Computation A) : Prop := eval c1 = eval c2.
+
+Theorem ceq_refl {A} (c : Computation A) : ceq c c.
+Proof.
+  reflexivity.
+Qed.
+
+Theorem ceq_sym {A} (c1 c2 : Computation A) : ceq c1 c2 -> ceq c2 c1.
+Proof.
+  unfold ceq.
+  intros.
+  auto.
+Qed.
+
+Theorem ceq_trans {A} (c1 c2 c3 : Computation A) : ceq c1 c2 -> ceq c2 c3 -> ceq c1 c3.
+Proof.
+  unfold ceq.
+  intros.
+  rewrite H.
+  auto.
+Qed.
+
+Theorem ret_inj : forall A a1 a2, ceq (ret A a1) (ret A a2) -> a1 = a2.
+Proof.
+  intros.
+  unfold ceq in H.
+  assert (forall x, eval (ret A x) = (fun a => a = x)). {
+    intros.
+    extensionality a.
+    apply propositional_extensionality.
+    split.
+    - intros.
+      inversion H0.
+      apply exist_inj2_uip in H3, H4.
+      subst.
+      reflexivity.
+    - intros.
+      subst.
+      constructor.
+  }
+  rewrite (H0 a1) in H.
+  rewrite (H0 a2) in H.
+  apply (f_equal (fun f => f a1)) in H.
+  rewrite <- H.
+  reflexivity.
+Qed.
+
+Theorem thing_thing : fancyid 3 = ret _ 3.
+Proof.
+  unfold fancyid.
+  simpl.
+  cbv cofix.
+
+Abort.
+
+CoInductive counit :=  nil : counit.
+
+Lemma unfold_counit : forall (n : counit), n = match n with nil => nil end.
+Proof.
+  intros.
+  destruct n.
+  reflexivity.
+Qed.
+
+Theorem even_simpler : (cofix id :=  nil ) = nil.
+Proof.
+  simpl.
+  rewrite unfold_counit at 1.
+  reflexivity.
+Qed.
+
+Theorem unfold_computation :
+  forall A (c : Computation A), c =
+                                  match c with
+                                  | ret A x => ret A x
+                                  | bind A B x f => bind A B x f
+                                  | multibind A B T x f => multibind A B T x f
+                                  end.
+Proof.
+Admitted.
+
+Theorem test_fun_fancyid : eval (fancyid 3) = eval (ret _ 3).
+Proof.
+  unfold fancyid.
+  rewrite unfold_computation at 1.
+  rewrite bindDef.
+
+(*
+
+
+(*
+f : nat * nat -> Prop
+f (0, _) = True
+f (n, S m) = not (forall n', f (n', m))
+ *)
+
+CoFixpoint f (n : nat) (m : nat) : Computation Prop :=
+  match m with
+  | O => ret _ True
+  | S m' => multibind _ _ nat (fun n' => f n' m') (fun rec => ret _ (not (forall n', rec n')))
+  end.
+ *)
+
+(* now, can I show that f 2 2 = True for example? *)
+
+Theorem test_run_f : eval (f 2 2) = eval (ret _ True).
+Proof.
+  unfold f.
+  
