theories/partial/partialBase.v
@@ -1,0 +1,291 @@
+Require Import Coq.Logic.ProofIrrelevance.
+(* Instead of using SProp, for now I'll just use the proof irrelevance axiom.
+   I'll see if this causes any issues; probably not. *)
+Require Import FunctionalExtensionality.
+Require Import Coq.Logic.PropExtensionality.
+
+Definition Partial (A : Type) : Type :=
+  {S : A -> Prop | forall x y, S x -> S y -> x = y}.
+
+
+Definition Preturn {A : Type} (x : A) : Partial A.
+  refine (exist _ (fun y => y = x) _).
+  intros.
+  congruence.
+Defined.
+
+Definition Pempty {A : Type} : Partial A.
+  refine (exist _ (fun x => False) _).
+  intros.
+  exfalso.
+  assumption.
+Defined.
+
+Theorem partialEq :
+  forall A S1 S2 p1 p2,
+    S1 = S2 -> @eq (Partial A) (exist _ S1 p1) (exist _ S2 p2).
+Proof.
+  intros.
+  subst S1.
+  assert (p1 = p2).
+  apply proof_irrelevance.
+  subst p1.
+  reflexivity.
+Qed.
+
+Theorem partialEq2:
+  forall A (x y : Partial A), proj1_sig x = proj1_sig y -> x = y.
+Proof.
+  intros.
+  destruct x.
+  destruct y.
+  simpl in H.
+  apply partialEq.
+  assumption.
+Qed.
+
+(* TODO: make better names for all these*)
+Theorem itIsReturn :
+  forall T (S : T -> Prop) (p : forall x y, S x -> S y -> x = y) (t : T),
+    S t -> (exist _ S p) = Preturn t.
+Proof.
+  intros.
+  apply partialEq.
+  apply functional_extensionality.
+  intros.
+  apply propositional_extensionality.
+  split.
+  - intros.
+    apply p.
+    assumption.
+    assumption.
+  - intros.
+    subst.
+    assumption.
+Qed.
+
+Theorem returnIsIt :
+  forall T (S : T -> Prop) (p : forall x y, S x -> S y -> x = y) (t : T),
+    (exist _ S p) = Preturn t
+    -> S t.
+Proof.
+  intros.
+  apply (@f_equal (Partial T) (T -> Prop) (@proj1_sig _ _) _ _) in H.
+  simpl in H.
+  rewrite H.
+  reflexivity.
+Qed.
+
+Theorem PreturnInj : forall A (x y : A), Preturn x = Preturn y -> x = y.
+Proof.
+  intros.
+  pose (@f_equal _ _ (@proj1_sig _ _) _ _ H) as fact.
+  simpl in fact.
+  assert ((fun y => y = x) x).
+  reflexivity.
+  rewrite fact in H0.
+  assumption.
+Qed.
+
+Definition Pbind {A B : Type} (pa : Partial A) (f : A -> Partial B) : Partial B.
+  refine (exist _ (fun b => exists a, proj1_sig pa a /\ proj1_sig (f a) b) _).
+  intros.
+  destruct H as [a temp].
+  destruct temp as [paa fax].
+  destruct H0 as [a' temp].
+  destruct temp as [paa' fa'y].
+  assert (aa' := proj2_sig pa a a' paa paa').
+  subst a'.
+  apply (proj2_sig (f a) x y fax fa'y).
+Defined.
+
+Theorem bindDef1 : forall A B {f : A -> Partial B}, Pbind Pempty f = Pempty.
+Proof.
+  intros.
+  apply partialEq.
+  apply functional_extensionality.
+  intros.
+  apply propositional_extensionality.
+  split.
+  - intros.
+    destruct H.
+    destruct H.
+    simpl in H.
+    assumption.
+  - intros. exfalso. assumption.
+Qed.
+
+Theorem bindDef2 : forall A B (a : A) (f : A -> Partial B),
+    Pbind (Preturn a) f = f a.
+Proof.
+  intros.
+  apply partialEq2.
+  apply functional_extensionality.
+  intros.
+  apply propositional_extensionality.
+  split.
+  - intros.
+    simpl in H.
+    destruct H.
+    destruct H.
+    subst x0.
+    assumption.
+  - intros.
+    simpl.
+    exists a.
+    split.
+    reflexivity.
+    assumption.
+Qed.
+
+Definition Pif {A : Type} (P : Prop) (a1 a2 : A) : Partial A.
+  refine (exist _ (fun a => (P /\ a = a1) \/ ((not P) /\ a = a2)) _).
+  intros.
+  destruct H.
+  destruct H.
+  destruct H0.
+  destruct H0.
+  subst.
+  reflexivity.
+  destruct H0.
+  contradiction.
+  destruct H.
+  destruct H0.
+  destruct H0.
+  contradiction.
+  destruct H0.
+  subst.
+  reflexivity.
+Defined.
+
+Theorem PifDef1 : forall (A : Type) P (a1 a2 : A), P -> Pif P a1 a2 = Preturn a1.
+Proof.
+  intros.
+  apply partialEq.
+  apply functional_extensionality.
+  intros.
+  apply propositional_extensionality.
+  split.
+  - intros.
+    destruct H0.
+    destruct H0.
+    assumption.
+    destruct H0.
+    contradiction.
+  - intros.
+    subst.
+    apply or_introl.
+    split.
+    assumption.
+    reflexivity.
+Qed.
+
+Theorem PifDef2 : forall (A : Type) P (a1 a2 : A), not P -> Pif P a1 a2 = Preturn a2.
+Proof.
+  intros.
+  apply partialEq.
+  apply functional_extensionality.
+  intros.
+  apply propositional_extensionality.
+  split.
+  - intros.
+    destruct H0.
+    + destruct H0.
+      contradiction.
+    + destruct H0.
+      assumption.
+  - intros.
+    subst.
+    apply or_intror.
+    split.
+    assumption.
+    reflexivity.
+Qed.
+(* Does multibind actually work? *)
+(* Maybe this will need (rest : (A -> Classical B) -> Partial C)*)
+Definition Pmultibind {A B C : Type} (f : A -> Partial B) (rest : (A -> B) -> Partial C) : Partial C.
+  (*refine (exist _ (fun c => forall (g : A -> B), (forall a, (Preturn (g a)) = f a) -> rest g = Preturn c) _).*)
+  refine (exist _ (fun c => exists (g : A -> B), (forall a, (Preturn (g a) = f a)) /\ rest g = Preturn c) _).
+  intros.
+  destruct H.
+  destruct H0.
+  destruct H.
+  destruct H0.
+  apply PreturnInj.
+  assert (x0 = x1). {
+    extensionality a.
+    specialize (H a).
+    specialize (H0 a).
+    rewrite <- H in H0.
+    apply PreturnInj in H0.
+    symmetry.
+    assumption.
+  }
+  subst.
+  rewrite <- H1.
+  rewrite <- H2.
+  reflexivity.
+Defined.
+
+Theorem multibindDef {A B C : Type} : forall f rest,
+    @Pmultibind A B C (fun a => Preturn (f a)) rest = rest f.
+Proof.
+  intros.
+  apply partialEq2.
+  extensionality c.
+  apply propositional_extensionality.
+  split.
+  - intros.
+    destruct H.
+    destruct H.
+    assert (x = f). {
+      extensionality a.
+      specialize (H a).
+      apply PreturnInj.
+      apply H.
+    }
+    subst.
+    rewrite H0.
+    simpl.
+    reflexivity.
+  - intros.
+    simpl.
+    exists f.
+    split.
+    + intros.
+      reflexivity.
+    + Check itIsReturn.
+      remember (rest f) as thing.
+      destruct thing.
+      simpl in H.
+      apply itIsReturn.
+      assumption.
+Qed.      
+
+
+(*This section is from https://proofassistants.stackexchange.com/questions/4696/how-to-extract-the-equality-between-the-second-projection-in-an-existential-in-c*)
+(* TODO: Is there really no easier way? Does this really require UIP? *)
+Section existT_inj2_uip.
+  Variables (A : Type) (P : A -> Type).
+
+  Implicit Type (x : A).
+  Print sigT.
+
+  Theorem exist_inj2_helper x (px : P x) (y : sigT P) :
+      @existT _ _ x px = y
+    -> exists e : x = projT1 y, eq_rect x P px _ e = projT2 y.
+  Proof using Type. intros []; exists eq_refl; auto. Qed.
+
+  Fact exists_inj2 x y (px : P x) (py : P y) :
+      existT _ x px = existT _ y py
+    -> exists e : x = y, eq_rect x P px _ e = py.
+  Proof using Type. intros (e & ?)%exist_inj2_helper. exists e; subst; simpl; auto. Qed.
+
+  Fact exist_inj2_uip :
+    forall x (p1 p2 : P x), existT _ x p1 = existT _ x p2 -> p1 = p2.
+  Proof using Type.
+    intros x p1 p2 (e & He)%exists_inj2.
+    rewrite (UIP _ _ _ e eq_refl) in He.
+    assumption.
+  Qed.
+End existT_inj2_uip.
