theories/partial/prog4.v
@@ -1,0 +1,152 @@
+Require Import Coq.Logic.ProofIrrelevance.
+Require Import FunctionalExtensionality.
+Require Import Coq.Logic.PropExtensionality.
+
+Require Import partialBase.
+
+
+Inductive Prog (A B : Type) : Type :=
+| Ret3 : Partial B -> Prog A B
+| Rec3 : forall (P : A -> Prop), ((forall a, P a -> B) -> Prog A B) -> Prog A B
+(* Unfortunately, the following won't work. It is necessary to be able to know the set of elements of A
+on which recursive calls are made. *)
+(*| Rec3' : ((A -> B) -> Prog3 A B) -> Prog3 A B*)
+.
+
+(*
+I doubt that this will work.
+How will I get recVals for recursive calls?
+The function may not even be computable.
+I could replace recVals with a relation or something, but the issue is the type of "rest".
+*)
+Inductive runProgR {A B : Type} (def : A -> Partial (Prog A B)) : Prog A B -> B -> Prop :=
+| retR3 : forall b, runProgR def (Ret3 _ _ (Preturn b)) b
+| recR3 : forall P (recVals : forall a, P a -> B)
+                 (res : B) (rest : (forall a, P a -> B) -> Prog A B),
+    (* if for all inputs a satisfying P, recVals describes the recursive calls *)
+    (forall a (pa : P a), exists prog,
+       def a = Preturn prog /\ runProgR def prog (recVals a pa))
+    (* and given the results of those recursive calls, the program outputs res *)
+    -> runProgR def (rest recVals) res
+    (* then overall res *)
+    -> runProgR def (Rec3 _ _ P rest) res
+.
+
+Theorem runProgFunction {A B : Type} {def : A -> Partial (Prog A B)} {p : Prog A B} {b1 b2 : B}
+  (rp1 : runProgR def p b1) (rp2 : runProgR def p b2) : b1 = b2.
+Proof.
+  intros.
+  generalize rp2.
+  generalize b2.
+  clear rp2.
+  clear b2.
+  induction rp1.
+  - intros.
+    inversion rp2.
+    subst.
+    apply (f_equal (fun f => f b)) in H0.
+    rewrite H0.
+    reflexivity.
+  - (* problem: why is there only 1 IH? There should be 1 for each of the recursive calls. *)
+    intros.
+    inversion rp2.
+    subst.
+    apply IHrp1.
+    assert (rest1 = rest). {
+      apply exist_inj2_uip in H1.
+      assumption.
+    }
+    subst.
+    assert (recVals = recVals0). {
+      extensionality a.
+      extensionality pa.
+      specialize (H a pa).
+      specialize (H2 a pa).
+      apply H1.
+      apply H5.
+    }
+    subst.
+    assumption.
+Qed.
+
+Definition runProgImpl3 {A B : Type} (def : A -> Partial (Prog3 A B)) (p : Prog3 A B) : Partial B.
+  refine (exist _ (fun b => runProg3R def p b) _).
+  intros.
+  assert (eq := runProgFunction3 H H0).
+  assumption.
+Defined.
+
+Definition runProg3 {A B : Type} (def : A -> Partial (Prog3 A B)) (a : A) : Partial B :=
+  Pbind (def a) (fun a' => 
+                   runProgImpl3 def a').
+
+Theorem runProgDefinitionRet3 {A B : Type} (def : A -> Partial (Prog3 A B)) (b : Partial B)
+  : runProgImpl3 def (Ret3 _ _ b) = b.
+Proof.
+  destruct b.
+  apply partialEq.
+  apply functional_extensionality.
+  intros b.
+  apply propositional_extensionality.
+  split.
+  - intros.
+    inversion H.
+    reflexivity.
+  - intros.
+    assert (exist _ x e = Preturn b). {
+      apply itIsReturn.
+      assumption.
+    }
+    rewrite H0.
+    apply retR3.
+    (* TODO: would this proof be simpler with definition proof irrelevance? *)
+Qed.
+
+Theorem runProgDefinitionRec3 {A B : Type} {def : A -> Partial (Prog3 A B)}
+        {P : A -> Prop}
+        {rest : (forall a, P a -> B) -> Prog3 A B}
+        {recVals : forall a, P a -> B}
+        {defVals : forall a, P a -> Prog3 A B}
+        (defValsCorrect : forall a (pa : P a), def a = Preturn (defVals a pa))
+        (recValsCorrect : forall a (pa : P a), runProg3 def a = Preturn (recVals a pa))
+  : runProgImpl3 def (Rec3 _ _ P rest) = runProgImpl3 def (rest recVals).
+Proof.
+  apply partialEq.
+  extensionality b.
+  apply propositional_extensionality.
+  split.
+  - intros.
+    inversion H.
+    subst.
+    apply exist_inj2_uip in H1.
+    subst.
+    assert (recVals = recVals0). {
+      extensionality a.
+      extensionality pa.
+      specialize (recValsCorrect a pa).
+      unfold runProg3 in recValsCorrect.
+      specialize (H2 a pa).
+      rewrite H2 in recValsCorrect.
+      rewrite bindDef2 in recValsCorrect.
+      apply returnIsIt in recValsCorrect.
+      specialize (H3 a pa).
+      assert (eq := runProgFunction3 recValsCorrect H3).
+      assumption.
+    }
+    subst.
+    assumption.
+  - intros.
+    Check @recR3.
+    Check (@recR3 _ _  def P recVals).
+    apply recR3 with (recVals := recVals) (defa := defVals).
+    assumption.
+    intros.
+    specialize (recValsCorrect a pa).
+    specialize (defValsCorrect a pa).
+    unfold runProg3 in recValsCorrect.
+    rewrite defValsCorrect in recValsCorrect.
+    rewrite bindDef2 in recValsCorrect.
+    apply returnIsIt in recValsCorrect.
+    assumption.
+    assumption.
+Qed.
