theories/unificationtest.v
@@ -1,0 +1,22 @@
+Require Import String.
+Require Import qterm.
+Require Import lambdaFacts.
+Require Import lambdaSolve.
+
+
+(* Can I recover first order unification on STLC types? *)
+
+Ltac solve_all := repeat (lambda_solve ; repeat neutral_inj_case ;lambda_solve
+                  ; repeat fast_neutral_unequal_case). 
+
+Theorem test1
+        (A B C : QTerm)
+        :
+        <Arrow `A `B> = <Arrow `B `C>
+        -> A = C.
+Proof.
+  intros.
+  solve_all.
+Qed.
+
+(* I guess obviously yes. *)
